QED Memory Safety for HMAC_SHA2_256

code/experimental/hmac/Hacl.Impl.HMAC_SHA2_256.fst
@@ -24,6 +24,7 @@ inline_for_extraction noextract
 let a = Spec.SHA2.SHA2_256
 
 
+
 (* Key wrapping function *)
 val wrap_key:
     output: lbuffer uint8 (Spec.SHA2.size_block a)
@@ -42,102 +43,91 @@ let wrap_key output key len =
   end
 
 
+#reset-options "--z3rlimit 25"
+
 val init:
-    hash: lbuffer uint32 Spec.SHA2.size_hash_w
+    state: lbuffer uint32 Spec.SHA2.size_hash_w
   -> key: lbuffer uint8 (Spec.SHA2.size_block a) ->
   Stack unit
-  (requires (fun h -> live h hash /\ live h key /\ disjoint hash key))
-  (ensures  (fun h0 _ h1 -> modifies1 key h0 h1))
+  (requires (fun h -> live h state /\ live h key /\ disjoint state key))
+  (ensures  (fun h0 _ h1 -> modifies1 state h0 h1))
 
-let init hash key =
+let init state key =
+  push_frame ();
+  let ipad = create (size (Spec.SHA2.size_block a)) (u8 0x36) in
+  let state' = create (size (Spec.SHA2.size_hash_w)) (u32 0) in
   let h0 = ST.get () in
-  salloc_nospec h0 (size (Spec.SHA2.size_block a)) (u8 0x36) (Ghost.hide (LowStar.Buffer.loc_buffer hash))
-  (fun ipad ->
-    let h0 = ST.get () in
-    loop_nospec #h0 (size (Spec.SHA2.size_block a)) ipad
-    (fun i -> ipad.(i) <- ipad.(i) ^. key.(i));
-
-    let hash' = create #uint32 #8 (size 8) (u32 0) in
-    (* let zeros = create #uint32 #8 (size 8) (u32 0) in *)
-    (* let ipad = create #uint8 #64 (size 64) (u8 0) in *)
-    Hash.init hash';
-    Hash.update_block hash' ipad;
-    copy hash (size 8) hash'
-    )
+  loop_nospec #h0 (size (Spec.SHA2.size_block a)) ipad
+  (fun i -> ipad.(i) <- ipad.(i) ^. key.(i));
+  Hash.init state';
+  Hash.update_block state' ipad;
+  copy state (size 8) state';
+  pop_frame ()
 
 
 val update_block:
-    hash: lbuffer uint32 Spec.SHA2.size_hash_w
+    state: lbuffer uint32 Spec.SHA2.size_hash_w
   -> block: lbuffer uint8 (Spec.SHA2.size_block a) ->
   Stack unit
-  (requires (fun h -> live h hash /\ live h block /\ disjoint hash block))
-  (ensures  (fun h0 _ h1 -> modifies1 hash h0 h1))
+  (requires (fun h -> live h state /\ live h block /\ disjoint state block))
+  (ensures  (fun h0 _ h1 -> modifies1 state h0 h1))
 
-let update_block hash block = Hacl.Impl.SHA2_256.update_block hash block
+let update_block state block = Hacl.Impl.SHA2_256.update_block state block
 
 
 val update_last:
-    hash: lbuffer uint32 Spec.SHA2.size_hash_w
+    state: lbuffer uint32 Spec.SHA2.size_hash_w
   -> prev: uint64
   -> last: buffer uint8
   -> len: size_t{ v len == length last
                /\ v len <= Spec.SHA2.size_block a
                /\ v len + uint_v prev <= Spec.SHA2.max_input a} ->
   Stack unit
-  (requires (fun h -> live h hash /\ live h last /\ disjoint hash last))
-  (ensures  (fun h0 _ h1 -> modifies1 hash h0 h1))
+  (requires (fun h -> live h state /\ live h last /\ disjoint state last))
+  (ensures  (fun h0 _ h1 -> modifies1 state h0 h1))
 
-let update_last hash prev last len = Hacl.Impl.SHA2_256.update_last hash prev last len
+let update_last state prev last len = Hacl.Impl.SHA2_256.update_last state prev last len
 
 
 val update:
-    hash: lbuffer uint32 Spec.SHA2.size_hash_w
+    state: lbuffer uint32 Spec.SHA2.size_hash_w
   -> input: buffer uint8
   -> len: size_t{ v len == length input
                /\ v len <= Spec.SHA2.max_input a} ->
   Stack unit
-  (requires (fun h -> live h hash /\ live h input /\ disjoint hash input))
-  (ensures  (fun h0 _ h1 -> modifies1 hash h0 h1))
+  (requires (fun h -> live h state /\ live h input /\ disjoint state input))
+  (ensures  (fun h0 _ h1 -> modifies1 state h0 h1))
 
-let update hash input len = Hacl.Impl.SHA2_256.update hash input len
+let update state input len = Hacl.Impl.SHA2_256.update state input len
 
-
-val finish:
-    hash: lbuffer uint8 (Spec.SHA2.size_hash a)
-  -> hw: lbuffer uint32 Spec.SHA2.size_hash_w
-  -> key: lbuffer uint8 (Spec.SHA2.size_block a) ->
-  Stack unit
-  (requires (fun h -> live h hash /\ live h key /\ live h hw
-                 /\ disjoint hash key /\ disjoint hash hw))
-  (ensures  (fun h0 _ h1 -> modifies1 key h0 h1))
 
 #set-options "--z3rlimit 50"
 
-let finish hash hw key =
+val finish:
+    hash: lbuffer uint8 (Spec.SHA2.size_hash a)
+  -> state: lbuffer uint32 Spec.SHA2.size_hash_w
+  -> key: lbuffer uint8 (Spec.SHA2.size_block a) ->
+  Stack unit
+  (requires (fun h -> live h hash /\ live h key /\ live h state
+                 /\ disjoint hash key /\ disjoint hash state))
+  (ensures  (fun h0 _ h1 -> modifies1 hash h0 h1))
+
+let finish hash state key =
+  push_frame();
+  let scratch = create (size (Spec.SHA2.size_block a) +. size (Spec.SHA2.size_hash a)) (u8 0x5c) in
+  let state2 = create (size Spec.SHA2.size_hash_w) (u32 0x00) in
+  let opad = sub #uint8 #(64 + 32) #64 scratch (size 0) (size (Spec.SHA2.size_block a)) in
+  let s4 = sub #uint8 #(64 + 32) #32 scratch (size (Spec.SHA2.size_block a)) (size (Spec.SHA2.size_hash a)) in
+  Hacl.Impl.SHA2_256.finish s4 state; (* s4 = hash *)
   let h0 = ST.get () in
-  salloc_nospec h0 (size (Spec.SHA2.size_block a) +. size (Spec.SHA2.size_hash a)) (u8 0x5c) (Ghost.hide (LowStar.Buffer.loc_buffer hash))
-  (fun scratch ->
-
-    let h1 = ST.get () in
-    salloc_nospec h1 (size Spec.SHA2.size_hash_w) (u32 0x00) (Ghost.hide (LowStar.Buffer.loc_union
-                                                                      (LowStar.Buffer.loc_buffer hash)
-                                                                      (LowStar.Buffer.loc_buffer scratch)))
-    (fun hw2 ->
-      let opad = sub #uint8 #(64 + 32) #64 scratch (size 0) (size (Spec.SHA2.size_block a)) in
-      let s4 = sub #uint8 #(64 + 32) #32 scratch (size (Spec.SHA2.size_block a)) (size (Spec.SHA2.size_hash a)) in
-      (* let block = create #uint8 #64 (size 64) (u8 0) in *)
-      (* let blockw = create #uint32 #8 (size 8) (u32 0) in *)
-      Hacl.Impl.SHA2_256.finish s4 hw; (* s4 = hash *)
-      let h0 = ST.get () in
-      loop_nospec #h0 (size (Spec.SHA2.size_block a)) opad
-      (fun i -> opad.(i) <- opad.(i) ^. key.(i)); (* s5 = opad *)
-      let s5 = opad in
-      Hacl.Impl.SHA2_256.init hw2;
-      Hacl.Impl.SHA2_256.update_block hw2 s5;
-      Hacl.Impl.SHA2_256.update_last hw2 (u64 (Spec.SHA2.size_block a)) s4 (size (Spec.SHA2.size_hash a));
-      Hacl.Impl.SHA2_256.finish hash hw2))
-
-
+  loop_nospec #h0 (size (Spec.SHA2.size_block a)) opad
+  (fun i -> opad.(i) <- opad.(i) ^. key.(i)); (* s5 = opad *)
+    let s5 = opad in
+  Hacl.Impl.SHA2_256.init state2;
+  Hacl.Impl.SHA2_256.update_block state2 s5;
+  Hacl.Impl.SHA2_256.update_last state2 (u64 (Spec.SHA2.size_block a)) s4 (size (Spec.SHA2.size_hash a));
+  Hacl.Impl.SHA2_256.finish hash state2;
+  pop_frame ()
 
 
 val hmac:
@@ -152,18 +142,13 @@ val hmac:
   (ensures  (fun h0 _ h1 -> modifies1 mac h0 h1))
 
 let hmac mac key klen input len =
-  let h0 = ST.get () in
-  salloc_nospec h0 (size (Spec.SHA2.size_block a)) (u8 0) (Ghost.hide (LowStar.Buffer.loc_buffer mac))
-  (fun okey ->
-    let h1 = ST.get () in
-    salloc_nospec h1 (size Spec.SHA2.size_hash_w) (u32 0) (Ghost.hide (LowStar.Buffer.loc_union
-                                                                      (LowStar.Buffer.loc_buffer mac)
-                                                                      (LowStar.Buffer.loc_buffer okey)))
-    (fun state ->
-      wrap_key okey key klen;
-      init state okey;
-      loopi_blocks_nospec (size (Spec.SHA2.size_block a)) len input
-      (fun i block state -> update_block state block)
-      (fun i len last state -> update_last state ((to_u64 i +. (u64 1)) *. u64 (Spec.SHA2.size_block a)) last len)
-      state;
-      finish mac state okey))
+  push_frame ();
+  let okey = create (size (Spec.SHA2.size_block a)) (u8 0) in
+  let state = create (size Spec.SHA2.size_hash_w) (u32 0) in
+  wrap_key okey key klen;
+  init state okey;
+  loopi_blocks_nospec (size (Spec.SHA2.size_block a)) len input
+  (fun i block state -> update_block state block)
+  (fun i len last state -> update_last state ((to_u64 i +. (u64 1)) *. u64 (Spec.SHA2.size_block a)) last len) state;
+  finish mac state okey;
+  pop_frame ()
